Common/CSets.v
@@ -273,25 +273,19 @@ WARN: FinSet (and LeibnizEquiv) typeclass needs to be either resolvable from
 (** * GSet Cartesian product ***)
 
 
-Section GSetProduct.
+Section GSetCProd.
   Context `{Countable A}.
   Context `{Countable B}.
 
-  Definition gset_product (sa : gset A) (sb : gset B) : gset (A * B) :=
-    set_fold (fun e1 res => res ∪ set_map (e1,.) sb) ∅ sa.
+  #[global] Instance gset_cprod : CProd (gset A) (gset B) (gset (A * B)) :=
+    λ sa sb, set_fold (fun e1 res => res ∪ set_map (e1,.) sb) ∅ sa.
 
-  (** × must be left associative because the * of types is left associative.
-      Thus if you have sa : gset A, sb : gset B and sc : gset C, then
-      sa × sb × sc : gset (A * B * C) *)
-  Infix "×" := gset_product (at level 44, left associativity) : stdpp_scope.
-
-  Lemma gset_product_spec (sa : gset A) (sb : gset B) a b :
+  Lemma gset_cprod_spec (sa : gset A) (sb : gset B) a b :
     (a, b) ∈ sa × sb ↔ a ∈ sa ∧ b ∈ sb.
-  Proof. unfold gset_product. funelim (set_fold _ _ _); set_solver. Qed.
+  Proof. unfold cprod, gset_cprod. funelim (set_fold _ _ _); set_solver. Qed.
 
-  Global Instance set_unfold_gset_product (sa : gset A) (sb : gset B) x P Q :
+  Global Instance set_unfold_gset_cprod (sa : gset A) (sb : gset B) x P Q :
     SetUnfoldElemOf x.1 sa P -> SetUnfoldElemOf x.2 sb Q ->
-    SetUnfoldElemOf x (sa × sb) (P /\ Q).
-  Proof using. tcclean. destruct x. apply gset_product_spec. Qed.
-End GSetProduct.
-Infix "×" := gset_product (at level 44, left associativity) : stdpp_scope.
+    SetUnfoldElemOf x (sa × sb) (P ∧ Q).
+  Proof using. tcclean. destruct x. apply gset_cprod_spec. Qed.
+End GSetCProd.
